generalized DH_KE ≤ C[DH_real]

theories/prob_eff_lang/probblaze/examples/DH_KE/DH_channel.v
@@ -200,57 +200,61 @@ Section handlee_verification.
                                                                      (iThySum (iThySum (SendAliceImpl γtoka γfraca γautha atokN) (RecvBobImpl γauthb))
                                                                         (iThySum (SendBobImpl γtokb γfracb γauthb btokN) (RecvAliceImpl γautha))).
  
+  Definition LblAuthChannel γtoka atokN γtokb btokN γfraca γfracb γautha γauthb : iLblThy Σ :=
+    [([channel1],[channel2], (iThySum (iThySum (SendAliceImpl γtoka γfraca γautha atokN) (RecvBobImpl γauthb))
+                                (iThySum (SendBobImpl γtokb γfracb γauthb btokN) (RecvAliceImpl γautha))))].
 
+  Definition LblAdv : iLblThy Σ :=  [([getKey1],[getKey2], (iThySum GetKey1 GetKey2))].
 
   (* Verification of DH_KE ≤ C[DH_real] *)
   (*------------------------------------------------------------*)
   
-  Lemma DH_KE_C_DH_real f1 f2 γtoka γtokb γfraca γfracb γautha γauthb :
-    let X' := X γtoka atokN γtokb btokN γfraca γfracb γautha γauthb in
-         is_closed_expr ∅ f1 →
-         is_closed_expr ∅ f2 →
-         token γtoka -∗
-         token γtokb -∗
-           own γautha (to_dfrac_agree (DfracOwn 1) #()%V) -∗
-           own γauthb (to_dfrac_agree (DfracOwn 1) #()%V) -∗
-           REL f1 ≤ f2 <|T|> {{ (λ v1 v2, ⌜v1 = #()%V ∧ v2 = #()%V⌝) }} -∗
-           REL (DH_KE getKey1 channel1 f1) ≤ (C getKey2 channel2 DH_real f2) <|X'|> {{ (λ v1 v2, ⌜ v1 = v2 ⌝) }}.
+  Lemma DH_KE_C_DH_real f1 f2 γtoka γtokb γfraca γfracb γautha γauthb L X :
+    let LblThy := LblAuthChannel γtoka atokN γtokb btokN γfraca γfracb γautha γauthb in
+    is_closed_expr ∅ f1 →
+    is_closed_expr ∅ f2 →
+    token γtoka -∗
+    token γtokb -∗
+    own γautha (to_dfrac_agree (DfracOwn 1) #()%V) -∗
+    own γauthb (to_dfrac_agree (DfracOwn 1) #()%V) -∗
+    BREL f1 ≤ f2 <|LblAdv ++ L|> {{ (λ v1 v2, ⌜v1 = #()%V ∧ v2 = #()%V⌝) }} -∗
+    BREL (DH_KE getKey1 channel1 f1) ≤ (C getKey2 channel2 DH_real f2) <|([getKey1], [getKey2], X) :: LblThy ++ L|> {{ (λ v1 v2, ⌜ v1 = v2 ⌝) }}.
   Proof using G.
-    iIntros (X' Hf1closed Hf2closed) "Htoka Htokb Ha Hb Hff".
-    iApply rel_alloctape_l. iIntros (α) "!> Hα". rel_pures_l.
-    iApply rel_alloctape_l. iIntros (β) "!> Hβ". rel_pures_l.
-    iApply rel_alloc_l. iIntros (la) "!> Hla".
-    iApply rel_alloc_l. iIntros (lb) "!> Hlb".
-    rel_pures_r. 
+    iIntros (LblThy Hf1closed Hf2closed) "Htoka Htokb Ha Hb Hff".
+    iApply brel_alloctape_l. iIntros (α) "!> Hα". brel_pures_l.
+    iApply brel_alloctape_l. iIntros (β) "!> Hβ". brel_pures_l.
+    iApply brel_alloc_l. iIntros (la) "!> Hla".
+    iApply brel_alloc_l. iIntros (lb) "!> Hlb".
+    brel_pures_r.
     do 3 rewrite subst_is_closed_empty; try done.
     iDestruct "Hα" as (ns) "(%Hf & Hα)". apply map_eq_nil in Hf. simplify_eq.
-    iApply rel_couple_TU; [done|]. iFrame. simpl. iIntros (a) "Hα".
+    iApply brel_couple_TU; [done|]. iFrame. simpl. iIntros (a) "Hα".
     iDestruct "Hβ" as (ms) "(%Hf' & Hβ)". apply map_eq_nil in Hf'. simplify_eq.
-    iApply rel_couple_TU; [done|]. iFrame "Hβ". simpl. iIntros (b) "Hβ".
-   
-    rel_pures_r. rewrite -Nat2Z.inj_mul.
-    do 3 rel_exp_r.
-    rel_pures_r.
+    iApply brel_couple_TU; [done|]. iFrame "Hβ". simpl. iIntros (b) "Hβ".
+
+    brel_pures_r. rewrite -Nat2Z.inj_mul.
+    do 3 brel_exp_r.
+    brel_pures_r.
     do 3 rewrite subst_is_closed_empty; try done.
-    rel_pures_l.
+    brel_pures_l.
     rewrite subst_is_closed_empty; last done.
-    
-    iApply fupd_rel.
+
+    iApply fupd_brel.
     set (ga := (g ^+ a)%g).
     iMod (auth_upd (vgval (g ^+ a)%g) with "Ha") as "Ha".
     iMod (auth_upd (vgval $ g ^+ b)%g with "Hb") as "Hb".
     iMod (auth_persist with "Ha") as "#Ha".
     iMod (auth_persist with "Hb") as "#Hb".
     iModIntro.
-  
-    iApply fupd_rel.
+
+    iApply fupd_brel.
     iMod (inv_alloc atokN _ (token γtoka ∨ own γfraca DfracDiscarded)%I with "[Htoka]") as "#Hinvta".
     { iNext; iLeft;iFrame. }
     iMod (inv_alloc btokN _ (token γtokb ∨ own γfracb DfracDiscarded)%I with "[Htokb]") as "#Hinvtb".
     { iNext; iFrame. }
     iModIntro.
     
-    iApply (rel_na_alloc
+    iApply (brel_na_alloc
               ((β ↪ (n; [b]) ∗ lb ↦ NONEV)
                ∨ (β ↪□ (n; [])
                   ∗ lb ↦□ SOMEV #b)
@@ -259,271 +263,243 @@ Section handlee_verification.
     iSplitL "Hβ Hlb"; [iNext; iFrame; iLeft; iFrame|].
     iIntros "#Hinvb".
     
-    iApply (rel_na_alloc
+    iApply (brel_na_alloc
               ((α ↪ (n; [a]) ∗ la ↦ NONEV)
                ∨ (α ↪□ (n; [])
                   ∗ la ↦□ SOMEV #a))%I
               alphaN).
     iSplitL "Hα Hla"; [iNext; iFrame; iLeft; iFrame|].
     iIntros "#Hinva".
-    
-    
-    iApply (rel_exhaustion [_] [_] _ _ with "[$]").
+
+    iDestruct (brel_introduction_mono _ (LblAdv ++ LblThy ++ L) with "[][$Hff]") as "Hff".
+    { iApply to_iThy_le_intro'. simpl. eapply submseteq_trans; last apply submseteq_swap. by apply submseteq_cons. }
+    iApply (brel_exhaustion with "[$]"); [done|done|].
+
     iLöb as "IH".
     
-    iSplit; [iIntros (v1 v2) "(-> & ->)"; rel_pures_l; by rel_pures_r|].
-    
-    iIntros (e1 e2 ?)
-      "[%e1' [%e2' [%k1 [%k2 [%S
-           (-> & %Hk1 & -> & %Hk2 & [(-> & -> & (#Hnone & #Hsome)) | (-> & -> & (#Hnone & #Hsome))] & #HQ)
-          ]]]]] #Hk".
-    
+    iSplit; [iIntros (v1 v2) "!# (-> & ->)"; by brel_pures|].
+    iIntros (?????) "!# %Hk1 %Hk2 [(-> & -> & #(Hnone & Hsome))|(-> & -> & #(Hnone & Hsome))] #Hcont".
+
     1 : {
-          do 2 rel_pures_l; [apply Hk1; set_solver|].
-          do 2rel_pures_r; [apply Hk2; set_solver|].
-          iApply (rel_na_inv _ _ alphaN ); [set_solver|].
-          iFrame "Hinva". 
-          iIntros "([(Hα & Hla) | (#Hα & #Hla)] & Hclose)".
-          - iApply (rel_load_l_mask [AppRCtx _; CaseCtx _ _]).
-            iFrame. iIntros "!> Hla". rel_pures_l.
-            iApply (rel_rand_l _ [AppRCtx _; AppRCtx _]).
-            iAssert (α ↪N (n; [fin_to_nat a]))%I with "[Hα]" as "Hα".
-            { iExists [a]. simpl. iFrame. done. }
-            iFrame. iIntros "!>Hα _". rel_pures_l.
-            iApply (rel_store_l _ _ _ [AppRCtx _; AppRCtx _] with "Hla").
-            iIntros "!> Hla".
-            rel_pures_l.
-            iApply (rel_exp_l _ [AppRCtx _]). rel_pures_l.
-     
-            iApply fupd_rel.
-            iMod (ghost_map_elem_persist with "Hla") as "#Hla".
-            iDestruct "Hα" as (ns) "(%Hf & Hα)". apply map_eq_nil in Hf. simplify_eq.
-            iMod (ghost_map_elem_persist with "Hα") as "#Hα".
-            iModIntro.
-            iApply rel_na_close. iFrame.
-            iSplitL; [iNext; iRight; iFrame "#"|].
-            
-           
-     
-            (* Send (gA, bob) *)
-            iApply (rel_bind' [_] [_]); [by iApply traversable_iThyTraverse|].
-            iApply rel_introduction'.
-            iExists _, _, [], [], _. do 2 (iSplit; [done|]; iSplit; [iPureIntro; apply _|]).
-            iSplitL; [|by iIntros "!>" (??) "H"; iApply "H"].
-            iLeft. iLeft. simpl.
-            iExists (vgval (g ^+ a)%g),  (vgval (g ^+ a)%g).
-            iSplitL.
-            { iMod (inv_acc with "Hinvta") as "([>Htok | >#Hfrac'] & Hclose)"; try done.
-              - iModIntro. iLeft.
-                iIntros. iFrame. iMod ("Hclose" with "[$]") as "_". iFrame "#". 
-                by iModIntro. 
-              - iModIntro. iRight. iFrame "#".
-                iApply "Hclose". iNext.
-                by iRight. }
-            iSplit; first ( do 2 (iSplit; try (iPureIntro; done))).
-            iModIntro.
-            
-            iApply rel_value.
-            rel_pures_l.
-            rel_pures_r.
-     
-            (* Recv bob (either none or some) *)
-            iApply (rel_bind' [_] [_]); [by iApply traversable_iThyTraverse|].
-            iApply rel_introduction'.
-            iExists _, _, [], [], _. do 2 (iSplit; [done|]; iSplit; [iPureIntro; apply _|]).
-            iSplitL; [|by iIntros "!>" (??) "H"; iApply "H"].
-            iLeft. iRight.
-            do 2 (iSplit; try (iPureIntro; done)).
-            iModIntro.
-            iSplitL.
-     
-            (* Recv bob = None *)
-            + iApply rel_value.
-              rel_pures_l. rel_pures_r.
-              iDestruct ("HQ" with "Hnone") as "HQfill".
-              iDestruct ("Hk" with "HQfill") as "Hfillrel".
-              iClear (Hk1 Hk2) "Hnone Hsome HQ Hk HQfill".
-     
-              (* First call is done. Can call getKey1 or getKey2 again. *)
-              iApply (rel_exhaustion [_] [_] _ _ with "[$]"). iApply "IH".
-     
-            (* Recv bob = Some gB *)
-            + iIntros (m) "Ha'".
-              iDestruct (auth_agree with "[$Hb] [$Ha']") as "<-".
-              iApply rel_value.
-              rel_pures_l. rel_exp_l. 
-              rel_pures_r.
-              rewrite -expgM. rewrite -ssrnat.multE.
-              rewrite -Nat.mul_comm.
-              
-              iDestruct ("HQ" with "Hsome") as "HQfill".
-              iDestruct ("Hk" with "HQfill") as "Hfillrel".
-              
-              (* First call is done. Can call getKey1 or getKey2 again. *)
-              iApply (rel_exhaustion [_] [_] _ _ with "[$]"). iApply "IH".
-              
-          - iApply rel_na_close. iFrame. iSplitL; [iRight; iFrame "#"|].
-            iApply (rel_load_l with "Hla"). iIntros "!> _". rel_pures_l. rel_exp_l. rel_pures_l.
-     
-             (* Send (gA, bob) *)
-            iApply (rel_bind' [AppRCtx _] [AppRCtx _]); [by iApply traversable_iThyTraverse|].
-            iApply rel_introduction'.
-            iExists _, _, [], [], _. do 2 (iSplit; [done|]; iSplit; [iPureIntro; apply _|]).
-            iSplitL; [|by iIntros "!>" (??) "H"; iApply "H"].
-            iLeft. iLeft.
-            iExists _, _.
-            iSplitL.
-            { iMod (inv_acc with "Hinvta") as "([>Htok | >#Hfrac'] & Hclose)"; try done.
-              - iModIntro. iLeft.
-                iIntros. iFrame. iMod ("Hclose" with "[$]") as "_". iFrame "#". 
-                by iModIntro. 
-              - iModIntro. iRight. iFrame "#".
-                iApply "Hclose". iNext.
-                by iRight. }
-            iSplit; first ( do 2 (iSplit; try (iPureIntro; done))).
-  
-            iModIntro. 
-            iApply rel_value.
-            rel_pures_l.
-            rel_pures_r.
-     
-            (* Recv bob (either none or some) *)
-            iApply (rel_bind' [_] [_]); [by iApply traversable_iThyTraverse|].
-            iApply rel_introduction'.
-            iExists _, _, [], [], _. do 2 (iSplit; [done|]; iSplit; [iPureIntro; apply _|]).
-            iSplitL; [|by iIntros "!>" (??) "H"; iApply "H"].
-            iLeft. iRight.
-            do 2 (iSplit; try (iPureIntro; done)).
-            iModIntro.
-            iSplitL.
-     
-            (* Recv bob = None *)
-            + iApply rel_value.
-              rel_pures_l. rel_pures_r.
-              iDestruct ("HQ" with "Hnone") as "HQfill".
-              iDestruct ("Hk" with "HQfill") as "Hfillrel".
-              iClear (Hk1 Hk2) "Hnone Hsome HQ Hk HQfill".
-     
-              (* First call is done. Can call getKey1 or getKey2 again. *)
-              iApply (rel_exhaustion [_] [_] _ _ with "[$]"). iApply "IH".
-     
-            (* Recv bob = Some gB *)
-            + iIntros (m) "Ha'".
-              iDestruct (auth_agree with "[$Hb] [$Ha']") as "<-".
-              iApply rel_value.
-              rel_pures_l. rel_exp_l. 
-              rel_pures_r.
-              rewrite -expgM. rewrite -ssrnat.multE.
-              rewrite -Nat.mul_comm.
-              
-              iDestruct ("HQ" with "Hsome") as "HQfill".
-              iDestruct ("Hk" with "HQfill") as "Hfillrel".
-              
-              (* First call is done. Can call getKey1 or getKey2 again. *)
-              iApply (rel_exhaustion [_] [_] _ _ with "[$]"). iApply "IH". }
-  
+      brel_pures; [apply Hk1; set_solver|apply Hk2; set_solver|].
+      iApply (brel_na_inv _ _ alphaN); first set_solver.
+      iFrame "Hinva".
+      iIntros "([(Hα & Hla) | (#Hα & #Hla)] & Hclose)".
+      - iApply (brel_load_l _ _ _ [AppRCtx _; CaseCtx _ _] with "[$]").
+        iIntros "!> Hla". brel_pures_l.
+        iApply (brel_rand_l _ [AppRCtx _;AppRCtx _]).
+        iAssert (α ↪N (n; [fin_to_nat a]))%I with "[Hα]" as "Hα".
+        { iExists [a]. simpl. iFrame. done. }
+        iFrame. iIntros "!>Hα _". brel_pures_l.
+        iApply (brel_store_l _ _ _ [AppRCtx _; AppRCtx _] with "[$]").
+        iIntros "!> Hla". brel_pures_l.
+        iApply (brel_exp_l [AppRCtx _]). brel_pures_l.
+
+        iApply fupd_brel.
+        iMod (ghost_map_elem_persist with "Hla") as "#Hla".
+        iDestruct "Hα" as (ns) "(%Hf & Hα)". apply map_eq_nil in Hf. simplify_eq.
+        iMod (ghost_map_elem_persist with "Hα") as "#Hα".
+        iModIntro.
+        iApply brel_na_close. iFrame.
+        iSplitL; [iNext; iRight; iFrame "#"|].
+
+        iApply (brel_bind' [_] [_]); [iApply traversable_to_iThy|].
+        iApply (brel_introduction' [channel1] [channel2]).
+        { apply elem_of_cons. right. apply elem_of_list_here. }
+
+        iExists _, _, [], [], _. do 2 (iSplit; [done|]; iSplit; [iPureIntro; apply _|]).
+        iSplitL; [|by iIntros "!>" (??) "H"; iApply "H"].
+        iLeft. iLeft. iExists _, _.
+        iSplitL.
+        { iMod (inv_acc with "Hinvta") as "([>Htok | >#Hfrac'] & Hclose)"; try done.
+          - iModIntro. iLeft.
+            iIntros. iFrame. iMod ("Hclose" with "[$]") as "_". iFrame "#". 
+            by iModIntro. 
+          - iModIntro. iRight. iFrame "#".
+            iApply "Hclose". iNext.
+            by iRight. }
+        iSplit; first ( do 2 (iSplit; try (iPureIntro; done))).
+        
+        iModIntro. 
+        iApply brel_value. iIntros "$ !>".
+        brel_pures.
+
+        iApply (brel_bind' [_] [_]); [iApply traversable_to_iThy|].
+        iApply (brel_introduction' [channel1] [channel2]).
+        { apply elem_of_cons. right. apply elem_of_list_here. }
+        iExists _, _, [], [], _. do 2 (iSplit; [done|]; iSplit; [iPureIntro; apply _|]).
+        iSplitL; [|by iIntros "!>" (??) "H"; iApply "H"].
+        iLeft. iRight.
+        do 2 (iSplit; try (iPureIntro; done)).
+        iModIntro.
+        iSplitL.
+
+        (* Recv bob = None *)
+        + iApply brel_value. iIntros "$ !>".
+          brel_pures.
+          iDestruct ("Hcont" with "Hnone") as "Hkk".
+          iApply (brel_exhaustion _ _ [_] [_] with "[$]"); [done|done|].
+          iApply "IH".
+
+        (* Recv bob = Some gB *)
+        + iIntros (m) "Ha'".
+          iDestruct (auth_agree with "[$Hb] [$Ha']") as "<-".
+          iApply brel_value. iIntros "$ !>".
+          brel_pures.
+          rewrite -expgM. rewrite -ssrnat.multE.
+          rewrite -Nat.mul_comm.
+          iDestruct ("Hcont" with "Hsome") as "Hkk".
+          iApply (brel_exhaustion _ _ [_] [_] with "[$]"); [done|done|].
+          iApply "IH".
+
+      - iApply brel_na_close. iFrame. iSplitL; [iRight; iFrame "#"|].
+        iApply (brel_load_l _ _ _ [AppRCtx _; CaseCtx _ _] with "[$]").
+        iIntros "!> _". brel_pures. brel_exp_l. brel_pures_l.
+
+        iApply (brel_bind' [_] [_]); [iApply traversable_to_iThy|].
+        iApply (brel_introduction' [channel1] [channel2]).
+        { apply elem_of_cons. right. apply elem_of_list_here. }
+        iExists _, _, [], [], _. do 2 (iSplit; [done|]; iSplit; [iPureIntro; apply _|]).
+        iSplitL; [|by iIntros "!>" (??) "H"; iApply "H"].
+        iLeft. iLeft.
+        iExists _, _.
+        iSplitL.
+        { iMod (inv_acc with "Hinvta") as "([>Htok | >#Hfrac'] & Hclose)"; try done.
+          - iModIntro. iLeft.
+            iIntros. iFrame. iMod ("Hclose" with "[$]") as "_". iFrame "#". 
+            by iModIntro. 
+          - iModIntro. iRight. iFrame "#".
+            iApply "Hclose". iNext.
+            by iRight. }
+        iSplit; first (iSplit; try (iPureIntro; done)).
+        iModIntro.
+        iApply brel_value. iIntros "$ !>".
+        brel_pures.
+        
+        iApply (brel_bind' [_] [_]); [iApply traversable_to_iThy|].
+        iApply (brel_introduction' [channel1] [channel2]).
+        { apply elem_of_cons. right. apply elem_of_list_here. }
+        iExists _, _, [], [], _. do 2 (iSplit; [done|]; iSplit; [iPureIntro; apply _|]).
+        iSplitL; [|by iIntros "!>" (??) "H"; iApply "H"].
+        iLeft. iRight.
+        do 2 (iSplit; try (iPureIntro; done)).
+        iModIntro.
+        iSplitL.
+
+        (* Recv bob = None *)
+        + iApply brel_value. iIntros "$ !>".
+          brel_pures.
+          iDestruct ("Hcont" with "Hnone") as "Hkk".
+          iApply (brel_exhaustion _ _ [_] [_] with "[$]"); [done|done|].
+          iApply "IH".
+
+        (* Recv bob = Some gB *)
+        + iIntros (m) "Ha'".
+          iDestruct (auth_agree with "[$Hb] [$Ha']") as "<-".
+          iApply brel_value. iIntros "$ !>".
+          brel_pures.
+          rewrite -expgM. rewrite -ssrnat.multE.
+          rewrite -Nat.mul_comm.
+          iDestruct ("Hcont" with "Hsome") as "Hkk".
+          iApply (brel_exhaustion _ _ [_] [_] with "[$]"); [done|done|].
+          iApply "IH". }
+
     1 : {
-           do 2 rel_pures_l; [apply Hk1; set_solver|]. 
-           do 2 rel_pures_r; [apply Hk2; set_solver|].
-           iApply (rel_bind' [_] [_]); [by iApply traversable_iThyTraverse|].
-           iApply rel_introduction'.
-           iExists _, _, [], [], _. do 2 (iSplit; [done|]; iSplit; [iPureIntro; apply _|]).
-           iSplitL; [|by iIntros "!>" (??) "H"; iApply "H"].
-           iRight. iRight.
-           do 2 (iSplit; try (iPureIntro; done)).
-           iModIntro.
-           iSplitL.
-           - iApply rel_value. 
-             rel_pures_l. rel_pures_r.
-             iDestruct ("HQ" with "Hnone") as "HQfill".
-             iDestruct ("Hk" with "HQfill") as "Hfillrel".
-             iClear (Hk1 Hk2) "Hnone Hsome HQ Hk HQfill".
-             iApply (rel_exhaustion [_] [_] _ _ with "[$]"). iApply "IH".
-           - iIntros (m) "Hb'".
-             iDestruct (auth_agree with "[$Ha] [$Hb']") as "<-".
-             iApply rel_value.
-             rel_pures_l. 
-             rel_pures_r.
+      brel_pures; [apply Hk1; set_solver|apply Hk2; set_solver|].
+      iApply (brel_bind' [_] [_]); [iApply traversable_to_iThy|].
+      iApply brel_introduction'.
+      { apply elem_of_cons. right. apply elem_of_list_here. }
+      iExists _, _, [], [], _. do 2 (iSplit; [done|]; iSplit; [iPureIntro; apply _|]).
+      iSplitL; [|by iIntros "!>" (??) "H"; iApply "H"].
+      iRight. iRight.
+      do 2 (iSplit; try (iPureIntro; done)).
+      iModIntro.
+      iSplitL.
+      { iApply brel_value. iIntros "$ !>".
+        brel_pures.
+        iDestruct ("Hcont" with "Hnone") as "Hkk".
+        iApply (brel_exhaustion _ _ [_] [_] with "[$]"); [done|done|].
+        iApply "IH". }
+      iIntros (m) "Hb'".
+      iDestruct (auth_agree with "[$Ha] [$Hb']") as "<-".
+      iApply brel_value. iIntros "$ !>".
+      brel_pures.
+      
+      iApply (brel_na_inv _ _ betaN ); [set_solver|].
+      iFrame "Hinvb". 
+      iIntros "(>[(Hβ & Hlb) | #(Hβ & Hlb)] & Hclose)".
+      - iApply (brel_load_l _ _ _ [AppRCtx _; CaseCtx _ _] with "[$]").
+        iIntros "!> Hlb". brel_pures_l.
+        iApply (brel_rand_l _ [AppRCtx _; AppRCtx _]).
+        iAssert (β ↪N (n; [fin_to_nat b]))%I with "[Hβ]" as "Hβ".
+        { iExists [b]. simpl. iFrame. done. }
+        iFrame. iIntros "!>Hβ _". brel_pures_l.
+        iApply (brel_store_l _ _ _ [AppRCtx _; AppRCtx _] with "Hlb").
+        iIntros "!> Hlb".
+        brel_pures. iApply (brel_exp_l [AppRCtx _]). brel_pures.
+
+        iApply fupd_brel.
+        iMod (ghost_map_elem_persist with "Hlb") as "#Hlb".
+        iDestruct "Hβ" as (ns) "(%Hf & Hβ)". apply map_eq_nil in Hf. simplify_eq.
+        iMod (ghost_map_elem_persist with "Hβ") as "#Hβ".
+        iModIntro.
+        iApply brel_na_close. iFrame.
+        iSplitL; [iRight; iFrame "#"|].
+
+        iApply (brel_bind' [AppRCtx _] [AppRCtx _]); [iApply traversable_to_iThy|].
+        iApply brel_introduction'. { apply elem_of_cons. right. apply elem_of_list_here. }
+        iExists _, _, [], [], _. do 2 (iSplit; [done|]; iSplit; [iPureIntro; apply _|]).
+        iSplitL; [|by iIntros "!>" (??) "H"; iApply "H"].
+        iRight. iLeft.
+        iExists _,_.
+        iSplitL.
+        { iMod (inv_acc with "Hinvtb") as "([>Htok | >#Hfrac'] & Hclose)"; try done.
+          - iModIntro. iLeft.
+            iIntros. iFrame. iMod ("Hclose" with "[$]") as "_". iFrame "#". 
+            by iModIntro. 
+          - iModIntro. iRight. iFrame "#".
+            iApply "Hclose". iNext.
+            by iRight. }
+        iSplit; first ( do 2 (iSplit; try (iPureIntro; done))).
+        iModIntro.
+
+        iApply brel_value. iIntros "$ !>".
+        brel_pures. brel_pures_l.
+        rewrite -expgM. rewrite -ssrnat.multE.
+        rewrite -Nat.mul_comm.
+
+        iDestruct ("Hcont" with "Hsome") as "Hkk".
+        iApply (brel_exhaustion _ _ [_] [_] with "[$]"); [done|done|].
+        iApply "IH".
+
+      - iApply brel_na_close. iFrame. iSplitL; [iRight; iFrame "#"|].
+        iApply (brel_load_l with "[$]").
+        iIntros "!> _". brel_pures_l. brel_exp_l. brel_pures.
+        iApply (brel_bind' [_] [_]); [iApply traversable_to_iThy|].
+        iApply brel_introduction'. { apply elem_of_cons. right. apply elem_of_list_here. }
+        iExists _, _, [], [], _. do 2 (iSplit; [done|]; iSplit; [iPureIntro; apply _|]).
+        iSplitL; [|by iIntros "!>" (??) "H"; iApply "H"].
+        iRight. iLeft.
+        iExists _,_.
+        iSplitL.
+        { iMod (inv_acc with "Hinvtb") as "([>Htok | >#Hfrac'] & Hclose)"; try done.
+          - iModIntro. iLeft.
+            iIntros. iFrame. iMod ("Hclose" with "[$]") as "_". iFrame "#". 
+            by iModIntro. 
+          - iModIntro. iRight. by iMod ("Hclose" with "[$]") as "_". }
+        iSplit; first ( do 2 (iSplit; try (iPureIntro; done))).
+        iModIntro.
+
+        iApply brel_value. iIntros "$ !>".
+        brel_pures.
+        rewrite -expgM. rewrite -ssrnat.multE.
+        rewrite -Nat.mul_comm.
+        iDestruct ("Hcont" with "Hsome") as "Hkk".
+        iApply (brel_exhaustion _ _ [_] [_] with "[$]"); [done|done|].
+        iApply "IH". }
+  Qed. 
+    
   
-             iApply (rel_na_inv _ _ betaN ); [set_solver|].
-             iFrame "Hinvb". 
-             iIntros "(>[(Hβ & Hlb) | #(Hβ & Hlb)] & Hclose)". 
-             + iApply (rel_load_l_mask [AppRCtx _; CaseCtx _ _]).
-               iFrame. iIntros "!> Hlb". rel_pures_l.
-               iApply (rel_rand_l _ [AppRCtx _; AppRCtx _]).
-               iAssert (β ↪N (n; [fin_to_nat b]))%I with "[Hβ]" as "Hβ".
-               { iExists [b]. simpl. iFrame. done. }
-               iFrame. iIntros "!>Hβ _". rel_pures_l.
-               iApply (rel_store_l _ _ _ [AppRCtx _; AppRCtx _] with "Hlb").
-               iIntros "!> Hlb".
-               rel_pures_l.
-               iApply (rel_exp_l _ [AppRCtx _]). rel_pures_l.
-  
-               iApply fupd_rel.
-               iMod (ghost_map_elem_persist with "Hlb") as "#Hlb".
-               iDestruct "Hβ" as (ns) "(%Hf & Hβ)". apply map_eq_nil in Hf. simplify_eq.
-               iMod (ghost_map_elem_persist with "Hβ") as "#Hβ".
-               iModIntro.
-               iApply rel_na_close. iFrame.
-               iSplitL; [iRight; iFrame "#"|].
-               
-               iApply (rel_bind' [AppRCtx _] [AppRCtx _]); [by iApply traversable_iThyTraverse|].
-               iApply rel_introduction'.
-               iExists _, _, [], [], _. do 2 (iSplit; [done|]; iSplit; [iPureIntro; apply _|]).
-               iSplitL; [|by iIntros "!>" (??) "H"; iApply "H"].
-               iRight. iLeft.
-               iExists _,_.
-               iSplitL.
-               { iMod (inv_acc with "Hinvtb") as "([>Htok | >#Hfrac'] & Hclose)"; try done.
-                 - iModIntro. iLeft.
-                   iIntros. iFrame. iMod ("Hclose" with "[$]") as "_". iFrame "#". 
-                   by iModIntro. 
-                 - iModIntro. iRight. iFrame "#".
-                   iApply "Hclose". iNext.
-                   by iRight. }
-               iSplit; first ( do 2 (iSplit; try (iPureIntro; done))).
-               iModIntro.
-  
-               iApply rel_value.
-               rel_pures_l. rel_pures_r.
-               rel_exp_l.
-               rewrite -expgM. rewrite -ssrnat.multE.
-               rewrite -Nat.mul_comm.
-               
-               iDestruct ("HQ" with "Hsome") as "HQfill".
-               iDestruct ("Hk" with "HQfill") as "Hfillrel".
-               
-               iApply (rel_exhaustion [_] [_] _ _ with "[$]"). iApply "IH".
-  
-             + iApply rel_na_close. iFrame. iSplitL; [iRight; iFrame "#"|].
-               iApply (rel_load_l with "Hlb"). iIntros "!> _". rel_pures_l. rel_exp_l. rel_pures_l.
-               
-               iApply (rel_bind' [AppRCtx _] [AppRCtx _]); [by iApply traversable_iThyTraverse|].
-               iApply rel_introduction'.
-               iExists _, _, [], [], _. do 2 (iSplit; [done|]; iSplit; [iPureIntro; apply _|]).
-               iSplitL; [|by iIntros "!>" (??) "H"; iApply "H"].
-               iRight. iLeft.
-               iExists _,_.
-               iSplitL.
-               { iMod (inv_acc with "Hinvtb") as "([>Htok | >#Hfrac'] & Hclose)"; try done.
-                 - iModIntro. iLeft.
-                   iIntros. iFrame. iMod ("Hclose" with "[$]") as "_". iFrame "#". 
-                   by iModIntro. 
-                 - iModIntro. iRight. by iMod ("Hclose" with "[$]") as "_". }
-               iSplit; first ( do 2 (iSplit; try (iPureIntro; done))).
-               iModIntro.
-  
-               iApply rel_value.
-               rel_pures_l. rel_pures_r.
-               rel_exp_l.
-               rewrite -expgM. rewrite -ssrnat.multE.
-               rewrite -Nat.mul_comm.
-               
-               iDestruct ("HQ" with "Hsome") as "HQfill".
-               iDestruct ("Hk" with "HQfill") as "Hfillrel".
-                
-               iApply (rel_exhaustion [_] [_] _ _ with "[$]"). iApply "IH". }
-  Qed.
 
   Lemma C_DH_real_DH_KE f1 f2 γtoka γtokb γfraca γfracb γautha γauthb :
     let X' := X γtoka atokN γtokb btokN γfraca γfracb γautha γauthb in
@@ -1824,3 +1800,5 @@ Section handlee_verification.
   Qed.
 
 End handlee_verification.
+
+                
